feat : ex1 termination & determinism of type check

mini-spec/ex1-func-and-var/ex1spec.v
@@ -21,7 +21,7 @@ Inductive type :=
 Inductive expr :=
     | NumE (n : nat)
     | BinE (op : binop) (exp1 exp2 : expr)
-    | LetE (x : id) (exp exp2 : expr)
+    | LetE (x : id) (exp1 exp2 : expr)
     | VarE (x : id)
     | FuncE (x : id) (ty : type) (exp : expr)
     | ApplyE (exp1 exp2 : expr).
@@ -65,3 +65,155 @@ Inductive Eval : environment -> expr -> value -> Prop :=
     | E_applyE : forall env ef ea x eb env_clo vala valr,
         (env |- ef ==> (CloV x eb env_clo)) -> (env |- ea ==> vala) -> (((x, vala) :: env_clo) |- eb ==> valr) -> env |- (ApplyE ef ea) ==> valr
 where "C |- e ==> t" := (Eval C e t).
+
+Fixpoint type_eq (ty1 ty2 : type) : bool := match ty1, ty2 with
+| INT, INT => true
+| Func ty11 ty12, Func ty21 ty22 => andb (type_eq ty11 ty21) (type_eq ty12 ty22)
+| _, _ => false
+end.
+
+Fixpoint type_check (C : context) (exp : expr) : option type :=
+    match exp with
+    | NumE n => Some INT
+    | BinE op exp1 exp2 =>
+        match (type_check C exp1), (type_check C exp2) with
+        | Some INT, Some INT => Some INT
+        | _, _ => None
+        end
+    | LetE x exp1 exp2 =>
+        match (type_check C exp1) with
+        | Some ty => type_check ((x, ty) :: C) exp2
+        | None => None
+        end
+    | VarE x => find_id x C
+    | FuncE x ty exp =>
+        match (type_check ((x, ty) :: C) exp) with
+        | Some ty_body => Some (Func ty ty_body)
+        | None => None
+        end
+    | ApplyE exp1 exp2 =>
+        match (type_check C exp1) with
+        | Some (Func ty1 ty2) =>
+            match (type_check C exp2) with
+            | Some ty1' => if type_eq ty1 ty1' then Some ty2 else None
+            | None => None
+            end
+        | _ => None
+        end
+    end.
+
+Theorem Termination_Type_Check :
+forall C exp typ, (C |- exp : typ) <-> type_check C exp = Some typ.
+Proof.
+    intros C exp typ.
+    split.
+    {
+        intro E. induction E; simpl; try (rewrite IHE1, IHE2); try reflexivity.
+        - rewrite H. reflexivity.
+        - rewrite IHE. reflexivity.
+        - assert (H : forall typ, type_eq typ typ = true). {
+            intro ty. induction ty.
+            + reflexivity.
+            + simpl. rewrite IHty1, IHty2. reflexivity.
+          }
+          specialize H with (typ := typ).
+          rewrite H. reflexivity.
+    }
+    {
+        generalize dependent typ. generalize dependent C.
+        induction exp; intros C typ E; simpl in E.
+        - injection E as E. rewrite <- E. apply T_numE.
+        - destruct (type_check C exp1) eqn:E1.
+            + destruct t.
+                ++ destruct (type_check C exp2) eqn:E2.
+                    +++ destruct t.
+                        ++++ injection E as E.
+                             rewrite <- E in *.
+                             assert (H1 : C |- exp1 : INT). {
+                                apply IHexp1. apply E1.
+                             }
+                             assert (H2 : C |- exp2 : INT). {
+                                apply IHexp2. apply E2.
+                             }
+                             apply T_binE; assumption.
+                        ++++ discriminate E. 
+                    +++ discriminate E.
+                ++ discriminate E.
+            + discriminate E.
+        - destruct (type_check C exp1) eqn:E1.
+            + apply IHexp1 in E1. apply IHexp2 in E. apply T_letE with (typ := t); assumption.
+            + discriminate E.
+        - apply T_varE; assumption.
+        - destruct (type_check ((x, ty) :: C) exp) eqn:E1.
+            + apply IHexp in E1. injection E as E. rewrite <- E. apply T_funcE; assumption.
+            + discriminate E.
+        - destruct (type_check C exp1) eqn:E1.
+            + destruct t.
+                ++ discriminate E.
+                ++ destruct (type_check C exp2) eqn:E2.
+                    +++ destruct (type_eq t1 t) eqn:E3.
+                        ++++ assert (H : forall ty1 ty2, type_eq ty1 ty2 = true -> ty1 = ty2). {
+                                intros ty1.
+                                induction ty1.
+                                + intros ty2 H. destruct ty2. reflexivity. discriminate.
+                                + intros ty2 H. destruct ty2. discriminate. simpl in H. f_equal.
+                                  - destruct (type_eq ty1_1 ty2_1) eqn:Eb1.
+                                    ++ apply IHty1_1 in Eb1. apply Eb1.
+                                    ++ discriminate H.
+                                  - destruct (type_eq ty1_1 ty2_1).
+                                    ++ destruct (type_eq ty1_2 ty2_2) eqn:Eb2.
+                                        +++ apply IHty1_2 in Eb2. apply Eb2.
+                                        +++ discriminate H.
+                                    ++ discriminate H.
+                            }
+                            apply H in E3. injection E as E. rewrite <- E.
+                            apply IHexp1 in E1. apply IHexp2 in E2. rewrite <- E3 in E2.
+                            apply T_applyE with (typ := t1); assumption.
+                        ++++ discriminate E.
+                    +++ discriminate E.
+            + discriminate E.
+    }
+Qed.
+
+(*
+Fixpoint evaluation (env : environment) (exp : expr) : option value :=
+    match exp with
+    | NumE n => Some (NumV n)
+    | BinE op exp1 exp2 =>
+        match (evaluation env exp1), (evaluation env exp2) with
+        | Some (NumV n1), Some (NumV n2) => 
+            match op with
+            | ADD => Some (NumV (n1 + n2))
+            | MUL => Some (NumV (n1 * n2))
+            end
+        | _, _ => None
+        end
+    | LetE x exp1 exp2 =>
+        match (evaluation env exp1) with
+        | Some val => evaluation ((x, val) :: env) exp2
+        | None => None
+        end
+    | VarE x => find_id x env
+    | FuncE x ty exp => Some (CloV x exp env)
+    | ApplyE exp1 exp2 =>
+        match (evaluation env exp1), (evaluation env exp2) with
+        | Some (CloV x exp env_clo), Some val => (evaluation ((x, val) :: env) exp)
+        | _, _ => None
+        end
+    end.
+Theorem Termination_Evaluation :
+forall env exp val, (env |- exp ==> val) <-> evaluation C exp = Some val.
+Admitted. 
+*)
+
+Theorem Determinism :
+forall C exp typ1 typ2, (C |- exp : typ1) -> (C |- exp : typ2) -> typ1 = typ2.
+Proof.
+    intros C exp typ1 typ2 E1.
+    generalize dependent typ2.
+    induction E1; intros typ2 E2; inversion E2; try reflexivity.
+    - apply IHE1_1 in H4. rewrite <- H4 in H5. apply IHE1_2 in H5. apply H5.
+    - rewrite H in H2. injection H2 as H2. apply H2.
+    - f_equal. apply IHE1 in H4. apply H4.
+    - apply IHE1_1 in H2. injection H2 as _ H2. apply H2.
+Qed.
